updating

specParNoCtxtSwitch/NonSpec.v
@@ -1,49 +1,78 @@
 Require Import AST. 
 Require Import Heap.
+Require Import Coq.Sets.Ensembles. 
 
 Definition pHeap := heap pivar_state. 
 
-Inductive ppool : Type :=
-  |pthread : pterm -> ppool
-  |pdot : ppool
-  |ppar : ppool -> ppool -> ppool.
+Definition pctxt := pterm -> pterm.
 
-Inductive pctxt : (pterm -> pterm) -> Prop :=
-|pBindCtxt : forall c N, pctxt c -> pctxt (fun M => pbind M N)
-|pHandleCtxt : forall c N, pctxt c -> pctxt (fun M => phandle M N)
+Inductive pvalue : pterm -> Prop :=
+|pretValue : forall M, pvalue (pret M)
+|praiseValue : forall M, pvalue (praise M)
+|pgetValue : forall i, pvalue (pget i)
+|pputValue : forall i M, pvalue (pput i M)
+|pdoneValue : forall M, pvalue (pdone M)
+|pnewValue : pvalue pnew
 .
+ 
+Inductive pdecompose : pterm -> pctxt -> pterm -> Prop :=
+|bindCtxt : forall E M N M', ~pvalue M -> pdecompose M E M' ->
+                           pdecompose (pbind M N) (fun x => pbind (E x) N) M'
+|bindCtxtValue : forall M N, pvalue M -> pdecompose (pbind M N) (fun x => x) (pbind M N)
+|handleCtxt : forall M M' N E,
+                ~pvalue M -> pdecompose M E M' ->
+                pdecompose (phandle M N) (fun x => phandle (E x) N) M'
+|handleCtxtValue : forall M N, pvalue M -> pdecompose (phandle M N) (fun x=>x) 
+                                                    (phandle M N)
+.
+Definition pPool := Ensemble pterm. 
+Definition pSingleton := Singleton pterm. 
+Definition pUnion := Union pterm. 
 
-Print pterm. 
-Inductive pstep : pHeap -> ppool -> pHeap -> ppool -> Prop :=
-|PBind : forall E t M N h T,
-              pctxt E -> t = E (pbind (pret M) N) ->
-              pstep h (ppar (pthread t) T) h (ppar (pthread (E (papp N M))) T)
+Inductive pstep : pHeap -> pPool -> pPool -> pHeap -> pPool -> pPool -> Prop :=
+|PBind : forall E t M N h T, 
+           pdecompose t E (pbind (pret M) N) -> 
+           pstep h T (pSingleton t) h T (pSingleton(E(papp N M)))
 |PBindRaise : forall E t M N h T,
-                   pctxt E -> t = E (pbind (praise M) N) ->
-                   pstep h (ppar (pthread t) T) h (ppar (pthread (E(praise M))) T)
-|PHandle : forall E t M N h T,
-             pctxt E -> t = E(phandle (praise M) N) ->
-             pstep h (ppar (pthread t) T) h (ppar (pthread (E (papp N M))) T)
-|PHandleRet : forall E t M N h T,
-                pctxt E -> t = E(phandle (pret M) N) ->
-                pstep h (ppar (pthread t) T) h (ppar (pthread (E (pret M))) T)
-|PFork : forall E t M T h,
-              pctxt E -> t = E (pfork M) ->
-              pstep h (ppar (pthread t) T) h (ppar (ppar (pthread (E (pret punit)))
-                                                         (pthread M)) T)
+                pdecompose t E (pbind (praise M) N) -> 
+                pstep h T (pSingleton t) h T (pSingleton (E(praise M)))
+|pHandle : forall E t M N h T,
+             pdecompose t E (phandle (praise M) N) -> 
+             pstep h T (pSingleton t) h T (pSingleton (E(papp N M)))
+|pHandleRet : forall E t M N h T,
+                pdecompose t E (phandle (pret M) N) -> 
+                pstep h T (pSingleton t) h T (pSingleton (E(pret M)))
+|pFork : forall E t M h T,
+           pdecompose t E (pfork M) -> 
+           pstep h T (pSingleton t) h (Add pterm T M) (pSingleton (E(pret punit)))
 |PGet : forall E M t h T x,
-             pctxt E -> t = E(pget x) -> heap_lookup x h = Some(pfull M) ->
-             pstep h (ppar (pthread t) T) h (ppar (pthread (E (pret M))) T)
+          heap_lookup x h = Some(pfull M) -> pdecompose t E (pget x) -> 
+          pstep h T (pSingleton t) h T (pSingleton (E(pret M)))
 |PPut : forall E t M h h' T x,
-             pctxt E -> t = E(pput x M) -> heap_lookup x h = Some pempty ->
-             h' = replace x (pfull M) h ->
-             pstep h (ppar (pthread t ) T) h' (ppar (pthread (E (pret punit))) T)
+          pdecompose t E (pput x M) -> heap_lookup x h = Some pempty ->
+          h' = replace x (pfull M) h ->
+          pstep h T (pSingleton t) (replace x (pfull M) h) T (pSingleton (E (pret punit)))
 |PNew : forall E t h h' T x,
-             pctxt E -> t = E pnew -> (x, h') = extend pempty h ->
-             pstep h (ppar (pthread t) T) h' (ppar (pthread (E(pret (pvar x)))) T)
-|PTerminate : forall h T M,
-                pstep h (ppar (pthread (pret M)) T) h (ppar pdot T)
+             pdecompose t E pnew -> (x, h') = extend pempty h ->
+             pstep h T (pSingleton t) h' T (pSingleton (E (pret (pvar x))))
+|PTerminate : forall h T M, pstep h T (pSingleton (pret M)) h T (Empty_set pterm)
+                
 .
+
+Inductive pmultistep : pHeap -> pPool -> pPool -> pHeap -> pPool -> pPool -> Prop :=
+|multi_refl : forall h p1 p2, pmultistep h p1 p2 h p1 p2
+|multi_step : forall T1 T2 T2' h h' h'' t t',
+                ~ In pterm T2 t -> pstep h (pUnion T1 T2) (pSingleton t) h' (pUnion T1 T2) t' ->
+                pmultistep h' T1 (pUnion T2 t') h'' T1 T2' ->
+                pmultistep h T1 (Add pterm T2 t) h'' T1 T2'
+.
+
+
+
+
+
+
+
 
 
 
