specParNoCtxtSwitch/NonSpecPureStep.v
@@ -1,0 +1,75 @@
+Require Import Spec. 
+Require Import NonSpec. 
+Require Import AST.
+Require Import Coq.Sets.Ensembles.   
+Require Import sets. 
+Require Import CpdtTactics. 
+Require Import SfLib. 
+
+Ltac applyHyp :=
+  match goal with
+      |H : forall a : _, ?X -> ?Y, H' : ?Z |- _ => apply H in H'
+  end. 
+
+Fixpoint alphaConvert t x y :=
+  match t with
+      |pivar z => if beq_nat x z then pivar y else t
+      |punit => punit
+      |ppair e1 e2 => ppair (alphaConvert e1 x y) (alphaConvert e2 x y)
+      |pvar z => if beq_nat x z then pvar y else t
+      |plambda z e => if beq_nat x z then plambda y (alphaConvert e x y) else plambda z (alphaConvert e x y)
+      |papp e1 e2 => papp (alphaConvert e1 x y) (alphaConvert e2 x y)
+      |pret e => pret (alphaConvert e x y)
+      |pbind e1 e2 => pbind (alphaConvert e1 x y) (alphaConvert e2 x y)
+      |pfork e => pfork (alphaConvert e x y)
+      |pnew => pnew
+      |pput z e => if beq_nat x y then pput y (alphaConvert e x y) else pput z (alphaConvert e x y)
+      |pget z => if beq_nat x y then pget y else t
+      |praise e => praise (alphaConvert e x y)
+      |phandle e1 e2 => phandle (alphaConvert e1 x y) (alphaConvert e2 x y)
+      |pdone e => pdone (alphaConvert e x y)
+      |pfst e => pfst (alphaConvert e x y)
+      |psnd e => psnd (alphaConvert e x y)
+  end. 
+
+Axiom alphaEqual : forall t x y t2, alphaConvert t x y = t2 -> t = t2. 
+
+Theorem termErasureDeterminsim : forall M T M1 M2,
+                                   eraseTerm M T M1 -> eraseTerm M T M2 -> M1 = M2. 
+Proof.
+  intros. generalize dependent M2. induction H; intros; try(inversion H0; reflexivity);
+  try(clear H; clear H0; match goal with
+                           |H:eraseTerm ?T ?T' ?M |- _ => 
+                            inversion H; clear H; applyHyp; applyHyp; subst; reflexivity
+                         end); 
+  try(clear H; match goal with
+                |H : eraseTerm ?T ?T' ?M |- _ =>
+                 inversion H; clear H; applyHyp; subst; reflexivity
+               end). 
+  {inversion H2. subst. apply IHeraseTerm1 in H5. apply IHeraseTerm2 in H6. 
+   subst. assert(pbind e1'0
+     (plambda i (pbind e2'0 (plambda j (pret (ppair (pvar i) (pvar j)))))) =
+   pbind e1'0
+     (plambda i (pbind e2'0 (plambda j0 (pret (ppair (pvar i0) (pvar j0))))))). 
+   apply alphaEqual with (x := j)(y := j0). simpl. 
+
+
+Theorem erasureDeterminism : forall t t1' t2' T, 
+                               eraseThread t T t1' -> eraseThread t T t2' -> t1' = t2'.
+Proof.
+  intros. inversion H. 
+  {subst. inversion H0. subst. 
+
+
+Theorem NonSpecPureStep : forall h h' sh sh' tid s1 s2 M tid' M' t t', 
+                            multistep h tEmptySet (tSingleton (tid, s1, s2, M)) h' 
+                                      tEmptySet (tSingleton(tid', s1, s2, M')) ->
+                            eraseThread (tid, s1, s2, M) tEmptySet (pSingleton t) ->
+                            eraseThread (tid', s1, s2, M') tEmptySet (pSingleton t') ->
+                            eraseHeap h sh -> eraseHeap h' sh' ->
+                            pmultistep sh (Empty_set pterm) (pSingleton t) sh' (Empty_set pterm) (pSingleton t'). 
+Proof.
+  intros. remember (tSingleton(tid, s1, s2, M)). remember (tSingleton (tid', s1, s2, M')).  induction H. 
+  {subst. inversion Heqe0. apply SingletonEq in H4. inversion H4. subst. 
+   
+
